hide uses of Pull behind an interface

share/pulse/examples/dice/cbor/CDDL.Spec.MapGroupGen2.fsti
@@ -732,7 +732,6 @@ val list_no_repeats_filter
   )
   [SMTPat (List.Tot.no_repeats_p (List.Tot.map fst (List.Tot.filter f l)))]
 
-(*
 val parser_spec_map_group
   (source0: det_map_group)
   (#source: det_map_group)
@@ -764,26 +763,6 @@ val parser_spec_map_group_eq
     parser_spec_map_group source0 p x == p x'
   ))
   [SMTPat (parser_spec_map_group source0 p x)]
-*)
-
-#restart-solver
-let parser_spec_map_group
-  (source0: det_map_group)
-  (#source: det_map_group)
-  (#source_fp: typ)
-  (#target: Type0)
-  (#target_size: target -> nat)
-  (p: map_group_parser_spec source source_fp target_size {
-    restrict_map_group source0 source /\
-    map_group_footprint source source_fp
-  })
-: Tot (parser_spec (t_map source0) (map_group_target_serializable target_size))
-= fun x ->
-    let Cbor.Map a = x in
-    let a' = List.Tot.filter (FStar.Ghost.Pull.pull (matches_map_group_entry source_fp any)) a in
-    ghost_map_split (FStar.Ghost.Pull.pull (matches_map_group_entry source_fp any)) (ghost_map_of_list a);
-    let res = p a' in
-    res
 
 let rec list_forall_memP_filter
   (#t: Type)
@@ -885,7 +864,6 @@ let map_group_serializer_spec_match_item_for
   ghost_map_equiv rem ghost_map_empty;
   res
 
-(*
 val map_group_parser_spec_concat
   (#source1: det_map_group)
   (#source_fp1: typ)
@@ -904,90 +882,9 @@ val map_group_parser_spec_concat
     (forall x . target_size x == target_size1 (fst x) + target_size2 (snd x))
   })
 : Tot (map_group_parser_spec (map_group_concat source1 source2) (source_fp1 `t_choice` source_fp2) target_size)
-*)
 
 #restart-solver
-let map_group_parser_spec_concat'
-  (#source1: det_map_group)
-  (#source_fp1: typ)
-  (#target1: Type)
-  (#target_size1: target1 -> nat)
-  (p1: map_group_parser_spec source1 source_fp1 target_size1)
-  (#source2: det_map_group)
-  (#source_fp2: typ)
-  (#target2: Type)
-  (#target_size2: target2 -> nat)
-  (p2: map_group_parser_spec source2 source_fp2 target_size2)
-  (target_size: (target1 & target2) -> nat {
-    map_group_footprint source1 source_fp1 /\
-    map_group_footprint source2 source_fp2 /\
-    typ_disjoint source_fp1 source_fp2 /\
-    (forall x . target_size x == target_size1 (fst x) + target_size2 (snd x))
-  })
-  (l: map_group_parser_spec_arg (map_group_concat source1 source2) (source_fp1 `t_choice` source_fp2))
-: Ghost (map_group_parser_spec_ret (map_group_concat source1 source2) (source_fp1 `t_choice` source_fp2) target_size l)
-    (requires True)
-    (ensures (fun l' ->
-        let f1 = FStar.Ghost.Pull.pull (matches_map_group_entry source_fp1 any) in
-        let f2 = FStar.Ghost.Pull.pull (matches_map_group_entry source_fp2 any) in
-        (forall x . f1 x == matches_map_group_entry source_fp1 any x) /\
-        (forall x . f2 x == matches_map_group_entry source_fp2 any x) /\ (
-        let l1 = List.Tot.filter f1 l in
-        let l2 = List.Tot.filter f2 l in
-        map_group_parser_spec_arg_prop source1 source_fp1 l1 /\
-        map_group_parser_spec_arg_prop source2 source_fp2 l2 /\
-        (l' <: (target1 & target2)) == ((p1 l1 <: target1), (p2 l2 <: target2))
-      )
-    ))
-=
-  ghost_map_equiv
-    (ghost_map_filter (FStar.Ghost.Pull.pull (matches_map_group_entry source_fp1 any)) (ghost_map_of_list l))
-    (ghost_map_filter (matches_map_group_entry source_fp1 any) (ghost_map_of_list l));
-  map_group_footprint_is_consumed source1 source_fp1 (ghost_map_of_list l);
-  let res1 = p1 (List.Tot.filter (FStar.Ghost.Pull.pull (matches_map_group_entry source_fp1 any)) l) in
-  let MapGroupDet c1 r1 = apply_map_group_det source1 (ghost_map_filter (matches_map_group_entry source_fp1 any) (ghost_map_of_list l)) in
-  ghost_map_disjoint_union_comm r1 (ghost_map_filter (matches_map_group_entry source_fp2 any) (ghost_map_of_list l));
-  ghost_map_split (matches_map_group_entry source_fp1 any) (ghost_map_of_list l);
-  let MapGroupDet c1' r1' = apply_map_group_det source1 (ghost_map_of_list l) in
-  ghost_map_equiv
-    (ghost_map_filter (notp_g (matches_map_group_entry source_fp1 any)) (ghost_map_of_list l))
-    (ghost_map_filter (matches_map_group_entry source_fp2 any) (ghost_map_of_list l));
-  map_group_footprint_consumed source1 source_fp1 (ghost_map_filter (matches_map_group_entry source_fp1 any) (ghost_map_of_list l)) (ghost_map_filter (matches_map_group_entry source_fp2 any) (ghost_map_of_list l));
-  ghost_map_union_assoc c1 r1 (ghost_map_filter (matches_map_group_entry source_fp2 any) (ghost_map_of_list l));
-  assert (r1' == r1 `ghost_map_union` ghost_map_filter (matches_map_group_entry source_fp2 any) (ghost_map_of_list l));
-  map_group_footprint_consumed source2 source_fp2 (ghost_map_filter (matches_map_group_entry source_fp2 any) (ghost_map_of_list l)) r1;
-  ghost_map_equiv
-    (ghost_map_filter (FStar.Ghost.Pull.pull (matches_map_group_entry source_fp2 any)) (ghost_map_of_list l))
-    (ghost_map_filter (matches_map_group_entry source_fp2 any) (ghost_map_of_list l));
-  let res2 = p2 (List.Tot.filter (FStar.Ghost.Pull.pull (matches_map_group_entry source_fp2 any)) l) in
-  ghost_map_length_disjoint_union
-    (ghost_map_of_list (List.Tot.filter (FStar.Ghost.Pull.pull (matches_map_group_entry source_fp1 any)) l))
-    (ghost_map_of_list (List.Tot.filter (FStar.Ghost.Pull.pull (matches_map_group_entry source_fp2 any)) l));
-  let res = (res1, res2) in
-  res
-
-let map_group_parser_spec_concat
-  (#source1: det_map_group)
-  (#source_fp1: typ)
-  (#target1: Type)
-  (#target_size1: target1 -> nat)
-  (p1: map_group_parser_spec source1 source_fp1 target_size1)
-  (#source2: det_map_group)
-  (#source_fp2: typ)
-  (#target2: Type)
-  (#target_size2: target2 -> nat)
-  (p2: map_group_parser_spec source2 source_fp2 target_size2)
-  (target_size: (target1 & target2) -> nat {
-    map_group_footprint source1 source_fp1 /\
-    map_group_footprint source2 source_fp2 /\
-    typ_disjoint source_fp1 source_fp2 /\
-    (forall x . target_size x == target_size1 (fst x) + target_size2 (snd x))
-  })
-: Tot (map_group_parser_spec (map_group_concat source1 source2) (source_fp1 `t_choice` source_fp2) target_size)
-= map_group_parser_spec_concat' p1 p2 target_size
-
-#restart-solver
-let map_group_parser_spec_concat_eq
+val map_group_parser_spec_concat_eq
   (#source1: det_map_group)
   (#source_fp1: typ)
   (#target1: Type)
@@ -1016,17 +913,6 @@ let map_group_parser_spec_concat_eq
     map_group_parser_spec_concat p1 p2 target_size l == (p1 l1, p2 l2)
   ))
   [SMTPat (map_group_parser_spec_concat p1 p2 target_size l)]
-= let f1 = FStar.Ghost.Pull.pull (matches_map_group_entry source_fp1 any) in
-  let f2 = FStar.Ghost.Pull.pull (matches_map_group_entry source_fp2 any) in
-  assert (
-    (forall x . f1 x == matches_map_group_entry source_fp1 any x) /\
-    (forall x . f2 x == matches_map_group_entry source_fp2 any x) /\ (
-    let l1 = List.Tot.filter f1 l in
-    let l2 = List.Tot.filter f2 l in
-    map_group_parser_spec_arg_prop source1 source_fp1 l1 /\
-    map_group_parser_spec_arg_prop source2 source_fp2 l2 /\
-    map_group_parser_spec_concat p1 p2 target_size l == (p1 l1, p2 l2)
-  ))
 
 let orp (#t: Type) (p1 p2: t -> bool) (x: t) : bool =
   p1 x || p2 x
