share/pulse/examples/dice/cbor/CDDL.Spec.MapGroupGen2.fst
@@ -1,0 +1,169 @@
+module CDDL.Spec.MapGroupGen2
+
+let map_group_footprint_concat_consumes_all_recip = admit ()
+
+let list_no_repeats_filter = admit ()
+
+#restart-solver
+let parser_spec_map_group'
+  (source0: det_map_group)
+  (#source: det_map_group)
+  (#source_fp: typ)
+  (#target: Type0)
+  (#target_size: target -> nat)
+  (p: map_group_parser_spec source source_fp target_size {
+    restrict_map_group source0 source /\
+    map_group_footprint source source_fp
+  })
+  (x: Cbor.raw_data_item { t_map source0 x })
+: Ghost target
+    (requires True)
+    (ensures (fun res ->
+      let f = FStar.Ghost.Pull.pull (matches_map_group_entry source_fp any) in
+      (forall x . Ghost.reveal f x == matches_map_group_entry source_fp any x) /\
+      (let x' = List.Tot.filter f (Cbor.Map?.v x) in
+      map_group_parser_spec_arg_prop source source_fp x' /\
+      res == p x'
+    )))
+=
+    let Cbor.Map a = x in
+    let a' = List.Tot.filter (FStar.Ghost.Pull.pull (matches_map_group_entry source_fp any)) a in
+    ghost_map_split (FStar.Ghost.Pull.pull (matches_map_group_entry source_fp any)) (ghost_map_of_list a);
+    let res = p a' in
+    res
+
+let parser_spec_map_group
+  source0 p
+= fun x -> parser_spec_map_group' source0 p x
+
+let parser_spec_map_group_eq
+  source0 #source #source_fp p x
+= let f = FStar.Ghost.Pull.pull (matches_map_group_entry source_fp any) in
+  assert (
+    (forall x . Ghost.reveal f x == matches_map_group_entry source_fp any x) /\
+    (let x' = List.Tot.filter f (Cbor.Map?.v x) in
+    map_group_parser_spec_arg_prop source source_fp x' /\
+    parser_spec_map_group source0 p x == p x'
+  ))
+
+#restart-solver
+let map_group_parser_spec_concat'
+  (#source1: det_map_group)
+  (#source_fp1: typ)
+  (#target1: Type)
+  (#target_size1: target1 -> nat)
+  (p1: map_group_parser_spec source1 source_fp1 target_size1)
+  (#source2: det_map_group)
+  (#source_fp2: typ)
+  (#target2: Type)
+  (#target_size2: target2 -> nat)
+  (p2: map_group_parser_spec source2 source_fp2 target_size2)
+  (target_size: (target1 & target2) -> nat {
+    map_group_footprint source1 source_fp1 /\
+    map_group_footprint source2 source_fp2 /\
+    typ_disjoint source_fp1 source_fp2 /\
+    (forall x . target_size x == target_size1 (fst x) + target_size2 (snd x))
+  })
+  (l: map_group_parser_spec_arg (map_group_concat source1 source2) (source_fp1 `t_choice` source_fp2))
+: Ghost (map_group_parser_spec_ret (map_group_concat source1 source2) (source_fp1 `t_choice` source_fp2) target_size l)
+    (requires True)
+    (ensures (fun l' ->
+        let f1 = FStar.Ghost.Pull.pull (matches_map_group_entry source_fp1 any) in
+        let f2 = FStar.Ghost.Pull.pull (matches_map_group_entry source_fp2 any) in
+        (forall x . f1 x == matches_map_group_entry source_fp1 any x) /\
+        (forall x . f2 x == matches_map_group_entry source_fp2 any x) /\ (
+        let l1 = List.Tot.filter f1 l in
+        let l2 = List.Tot.filter f2 l in
+        map_group_parser_spec_arg_prop source1 source_fp1 l1 /\
+        map_group_parser_spec_arg_prop source2 source_fp2 l2 /\
+        (l' <: (target1 & target2)) == ((p1 l1 <: target1), (p2 l2 <: target2))
+      )
+    ))
+=
+  ghost_map_equiv
+    (ghost_map_filter (FStar.Ghost.Pull.pull (matches_map_group_entry source_fp1 any)) (ghost_map_of_list l))
+    (ghost_map_filter (matches_map_group_entry source_fp1 any) (ghost_map_of_list l));
+  map_group_footprint_is_consumed source1 source_fp1 (ghost_map_of_list l);
+  let res1 = p1 (List.Tot.filter (FStar.Ghost.Pull.pull (matches_map_group_entry source_fp1 any)) l) in
+  let MapGroupDet c1 r1 = apply_map_group_det source1 (ghost_map_filter (matches_map_group_entry source_fp1 any) (ghost_map_of_list l)) in
+  ghost_map_disjoint_union_comm r1 (ghost_map_filter (matches_map_group_entry source_fp2 any) (ghost_map_of_list l));
+  ghost_map_split (matches_map_group_entry source_fp1 any) (ghost_map_of_list l);
+  let MapGroupDet c1' r1' = apply_map_group_det source1 (ghost_map_of_list l) in
+  ghost_map_equiv
+    (ghost_map_filter (notp_g (matches_map_group_entry source_fp1 any)) (ghost_map_of_list l))
+    (ghost_map_filter (matches_map_group_entry source_fp2 any) (ghost_map_of_list l));
+  map_group_footprint_consumed source1 source_fp1 (ghost_map_filter (matches_map_group_entry source_fp1 any) (ghost_map_of_list l)) (ghost_map_filter (matches_map_group_entry source_fp2 any) (ghost_map_of_list l));
+  ghost_map_union_assoc c1 r1 (ghost_map_filter (matches_map_group_entry source_fp2 any) (ghost_map_of_list l));
+  assert (r1' == r1 `ghost_map_union` ghost_map_filter (matches_map_group_entry source_fp2 any) (ghost_map_of_list l));
+  map_group_footprint_consumed source2 source_fp2 (ghost_map_filter (matches_map_group_entry source_fp2 any) (ghost_map_of_list l)) r1;
+  ghost_map_equiv
+    (ghost_map_filter (FStar.Ghost.Pull.pull (matches_map_group_entry source_fp2 any)) (ghost_map_of_list l))
+    (ghost_map_filter (matches_map_group_entry source_fp2 any) (ghost_map_of_list l));
+  let res2 = p2 (List.Tot.filter (FStar.Ghost.Pull.pull (matches_map_group_entry source_fp2 any)) l) in
+  ghost_map_length_disjoint_union
+    (ghost_map_of_list (List.Tot.filter (FStar.Ghost.Pull.pull (matches_map_group_entry source_fp1 any)) l))
+    (ghost_map_of_list (List.Tot.filter (FStar.Ghost.Pull.pull (matches_map_group_entry source_fp2 any)) l));
+  let res = (res1, res2) in
+  res
+
+let map_group_parser_spec_concat
+  (#source1: det_map_group)
+  (#source_fp1: typ)
+  (#target1: Type)
+  (#target_size1: target1 -> nat)
+  (p1: map_group_parser_spec source1 source_fp1 target_size1)
+  (#source2: det_map_group)
+  (#source_fp2: typ)
+  (#target2: Type)
+  (#target_size2: target2 -> nat)
+  (p2: map_group_parser_spec source2 source_fp2 target_size2)
+  (target_size: (target1 & target2) -> nat {
+    map_group_footprint source1 source_fp1 /\
+    map_group_footprint source2 source_fp2 /\
+    typ_disjoint source_fp1 source_fp2 /\
+    (forall x . target_size x == target_size1 (fst x) + target_size2 (snd x))
+  })
+: Tot (map_group_parser_spec (map_group_concat source1 source2) (source_fp1 `t_choice` source_fp2) target_size)
+= map_group_parser_spec_concat' p1 p2 target_size
+
+#restart-solver
+let map_group_parser_spec_concat_eq
+  (#source1: det_map_group)
+  (#source_fp1: typ)
+  (#target1: Type)
+  (#target_size1: target1 -> nat)
+  (p1: map_group_parser_spec source1 source_fp1 target_size1)
+  (#source2: det_map_group)
+  (#source_fp2: typ)
+  (#target2: Type)
+  (#target_size2: target2 -> nat)
+  (p2: map_group_parser_spec source2 source_fp2 target_size2)
+  (target_size: (target1 & target2) -> nat {
+    map_group_footprint source1 source_fp1 /\
+    map_group_footprint source2 source_fp2 /\
+    typ_disjoint source_fp1 source_fp2 /\
+    (forall x . target_size x == target_size1 (fst x) + target_size2 (snd x))
+  })
+  (l: map_group_parser_spec_arg (map_group_concat source1 source2) (source_fp1 `t_choice` source_fp2))
+: Lemma
+  (exists (f1: _ -> bool) (f2: _ -> bool) .
+    (forall x . f1 x == matches_map_group_entry source_fp1 any x) /\
+    (forall x . f2 x == matches_map_group_entry source_fp2 any x) /\ (
+    let l1 = List.Tot.filter f1 l in
+    let l2 = List.Tot.filter f2 l in
+    map_group_parser_spec_arg_prop source1 source_fp1 l1 /\
+    map_group_parser_spec_arg_prop source2 source_fp2 l2 /\
+    map_group_parser_spec_concat p1 p2 target_size l == (p1 l1, p2 l2)
+  ))
+  [SMTPat (map_group_parser_spec_concat p1 p2 target_size l)]
+= let f1 = FStar.Ghost.Pull.pull (matches_map_group_entry source_fp1 any) in
+  let f2 = FStar.Ghost.Pull.pull (matches_map_group_entry source_fp2 any) in
+  assert (
+    (forall x . f1 x == matches_map_group_entry source_fp1 any x) /\
+    (forall x . f2 x == matches_map_group_entry source_fp2 any x) /\ (
+    let l1 = List.Tot.filter f1 l in
+    let l2 = List.Tot.filter f2 l in
+    map_group_parser_spec_arg_prop source1 source_fp1 l1 /\
+    map_group_parser_spec_arg_prop source2 source_fp2 l2 /\
+    map_group_parser_spec_concat p1 p2 target_size l == (p1 l1, p2 l2)
+  ))
